dev2020/dsubsup_cc/d2cc2.v
@@ -1,0 +1,329 @@
+Require Import List.
+
+Infix "\o" := (fun f g x => f (g x)) (at level 50).
+
+Module Cx.
+  Section var.
+    Context {var ty : Type}.
+    Hypothesis lem_var : forall x y : var, {x = y} + {x <> y}.
+
+    Definition t : Type := list (var * ty).
+
+    Inductive lookup : t -> var -> ty -> Prop :=
+      | top : forall {G x T}, lookup ((x, T) :: G) x T
+      | pop : forall {G x T}, lookup G x T -> 
+              forall {y U}, x <> y -> lookup ((y, U) :: G) x T.
+
+    Definition isFresh (G : t) (x : var) : Prop := forall T, ~ lookup G x T.
+    Definition eq (G D : t) := forall x T, lookup G x T <-> lookup D x T.
+
+  End var.
+End Cx.
+
+Module Result.
+
+  Inductive t (X : Type) := 
+    | Ok : X -> nat -> t X
+    | Fail : t X
+    | NoFuel : t X.
+
+  Definition bind {X} (u : t X) {Y} (f : X -> nat -> t Y) : t Y :=
+    match u with
+    | Ok _ x n => f x n
+    | Fail _ => Fail _
+    | NoFuel _ => NoFuel _
+    end.
+
+End Result.
+
+Notation "'do' x , n <- e ; u" := (Result.bind e (fun n x => u))
+  (at level 200, x ident, n ident, e at level 100, u at level 200).
+
+Module CC.
+  (* We're adopting the Theory of Contexts. Thus, we parameterize over all
+     variables and postulate decidable equality. *)
+  Parameter var : Type.
+  Hypothesis lem_var : forall x y : var, {x = y} + {x <> y}.
+
+  Definition beq_var (x y : var) : bool :=
+    match lem_var x y with
+    | left _ => true
+    | right _ => false
+    end.
+
+  (* Presyntax *)
+  Inductive sort : Type := prop | type.
+
+  Inductive expr : Type :=
+    | TSort : sort -> expr
+    | tVar : var -> expr
+    | TAll : expr -> (var -> expr) -> expr
+    | tLam : (var -> expr) -> expr
+    | tApp : expr -> expr -> expr
+    | TSig : expr -> (var -> expr) -> expr
+    | tPair : expr -> expr -> expr
+    | tFst : expr -> expr
+    | tSnd : expr -> expr.
+
+  Definition cx : Type := @Cx.t var expr.
+
+  Coercion TSort : sort >-> expr.
+  Coercion tVar : var >-> expr.
+
+  (* The Theory of Contexts is actually a theory about term contexts, or
+     holes. *)
+  Fixpoint hole (n : nat) : Type :=
+    match n with
+    | 0 => expr
+    | S n' => var -> hole n'
+    end.
+
+  Inductive isFresh (x : var) : forall n, hole n -> Prop :=
+    | fr_sort : forall s : sort, isFresh x 0 s
+    | fr_var : forall y, x <> y -> isFresh x 0 y
+    | fr_all : forall T U, 
+        isFresh x 0 T -> isFresh x 1 U -> isFresh x 0 (TAll T U)
+    | fr_lam : forall t, isFresh x 1 t -> isFresh x 0 (tLam t)
+    | fr_app : forall t u, 
+        isFresh x 0 t -> isFresh x 0 u -> isFresh x 0 (tApp t u)
+    | fr_sig : forall T U, 
+        isFresh x 0 T -> isFresh x 1 U -> isFresh x 0 (TSig T U)
+    | fr_pair : forall t u, 
+        isFresh x 0 t -> isFresh x 0 u -> isFresh x 0 (tPair t u)
+    | fr_fst : forall t, isFresh x 0 t -> isFresh x 0 (tFst t)
+    | fr_snd : forall t, isFresh x 0 t -> isFresh x 0 (tSnd t)
+    | fr_hole : forall e y, isFresh x 0 (e y) -> isFresh x 0 y -> isFresh x 1 e.
+
+  Hypothesis freshVarP : forall {n} e, sig (fun x => isFresh x n e).
+  Definition freshVar {n} (e : hole n) : var := proj1_sig (freshVarP e).
+
+  (* Holes are actually monads on variable representation in non-dependently 
+     typed systems. They are almost monads in our dependently typed language. *)
+  Fixpoint flatMap {n} (f : var -> hole n) {m} : hole m -> hole (n + m).
+  Abort.
+  (* But we don't need that kind of expressive power for now. Let's settle for 
+     this slightly less powerful function. *)
+  Fixpoint flatMap (f : var -> expr) (e : expr) : expr :=
+    match e with
+    | TSort s => TSort s
+    | tVar x => f x
+    | TAll T U => TAll (flatMap f T) (flatMap f \o U)
+    | tLam t => tLam (flatMap f \o t)
+    | tApp t u => tApp (flatMap f t) (flatMap f u)
+    | TSig T U => TSig (flatMap f T) (flatMap f \o U)
+    | tPair t u => tPair (flatMap f t) (flatMap f u)
+    | tFst t => tFst (flatMap f t)
+    | tSnd t => tSnd (flatMap f t)
+    end.
+
+  Definition subst (x : var) (e : expr) : var -> expr := 
+    fun y => if beq_var x y then e else y.
+  Notation "[ e \ x ]" := (flatMap (subst x e)) (at level 50).
+
+  Definition close (x : var) (e : expr) : var -> expr := fun y => [y \ x] e.
+
+  (*
+  (* Postulate unsaturation? *)
+  Fixpoint eval (fuel : nat) (e : expr) : Result.t (expr * nat).
+  Proof.
+    refine(
+    match fuel with
+    | 0 => Result.NoFuel _
+
+    | S fuel' =>
+        match e with
+        | TSort s => 
+          Result.Ok _ (TSort s) fuel'
+
+        | tVar x => 
+          Result.Ok _ (tVar x) fuel'
+
+        | TAll T U =>
+          do T', n1 <- eval fuel' T;
+          let x := freshVar U in
+          do U', n2 <- eval1 n (U x);
+          Result.Ok _ (TAll T' (close x U')) n2
+
+        | tLam t => 
+          let x := freshVar t in
+          do t', n <- eval fuel' (t x);
+          Result.Ok _ (tLam (close x t')) n
+
+        | tApp t u => 
+          do t', n1 <- eval fuel' t;
+          match t' with
+          | tLam w =>
+            do u', n2 <- eval n1 u;
+            _
+
+          | _ => Result.Fail _
+          end
+
+        | TSig T U => 
+          do T', n1 <- eval fuel' T;
+          let x := freshVar U' in
+          do U', n2 <- eval n1 (U x);
+          Result.Ok _ (TSig T' (close x U')) n2
+
+        | tPair t u => 
+          do t', n1 <- eval fuel' t;
+          do u', n2 <- eval n1 u;
+          Result.Ok _ (tPair t' u') n2
+
+        | tFst t => 
+          do t', n <- eval fuel' t;
+          match (fst tk) with
+          | tPair u _ => 
+            if n >=? 0 then Result.Ok _ 
+
+          | _ => Result.Fail _
+          end
+
+        | tSnd t => 
+          do tk <- eval fuel' t;
+          match (fst tk) with
+          | tPair _ u =>
+            Result.Ok _ (u, snd tk)
+
+          | _ => Result.Fail _
+          end
+        end
+     end).
+  Proof.
+
+  Inductive step : expr -> expr -> Prop :=
+    | r_beta : forall t u x, step (tApp (tLam t) u) ([u \ ])
+   *)
+  
+  Definition Eq (e u : expr) : Prop := True.
+
+  Inductive Cx : cx -> Prop :=
+    | Nil : Cx nil
+
+    | Snoc : forall {G T x s},
+        Expr G T (TSort s) ->
+        Cx.isFresh G x ->
+        Cx ((x, T) :: G)
+
+    with Expr : cx -> expr -> expr -> Prop :=
+    | TyAx : forall {G}, Cx G -> Expr G prop type
+    | tmVar : forall {G x T}, Cx G -> Cx.lookup G x T -> Expr G x T
+
+    | TyAll : forall {G T s U s' x},
+        Expr G T (TSort s) ->
+        Expr ((x, T) :: G) (U x) (TSort s') ->
+        Cx.isFresh G x -> (* Do we need this? *)
+        Expr G (TAll T U) (TSort s')
+
+    | tmLam : forall {G T s t U x},
+        Expr G T (TSort s) ->
+        Expr ((x, T) :: G) (t x) (U x) ->
+        Cx.isFresh G x -> (* Do we need this? *)
+        Expr G (tLam t) (TAll T U)
+
+    | tmApp : forall {G t T U u x},
+        Expr G t (TAll T U) ->
+        Expr G u T ->
+        Cx.isFresh G x -> (* Do we need this? *)
+        Expr G (tApp t u) ([u \ x] (U x))
+
+    | TySig : forall {G T s U s' x},
+        Expr G T (TSort s) ->
+        Expr ((x, T) :: G) (U x) (TSort s') ->
+        Cx.isFresh G x -> (* Do we need this? *)
+        Expr G (TSig T U) (TSort s')
+
+    | tmPair : forall {G T U s t u x},
+        Expr G (TSig T U) (TSort s) ->
+        Expr G t T ->
+        Expr G u ([t \ x] (U x)) ->
+        Cx.isFresh G x ->
+        Expr G (tPair t u) (TSig T U)
+
+    | tmFst : forall {G t T U},
+        Expr G t (TSig T U) ->
+        Expr G (tFst t) T
+
+    | tmSnd : forall {G t T U x},
+        Expr G t (TSig T U) ->
+        Cx.isFresh G x ->
+        Expr G (tSnd t) ([tFst t \ x] (U x))
+
+    | tmConv : forall {G e T U s},
+        Expr G e T ->
+        Eq T U ->
+        Expr G U (TSort s) ->
+        Expr G e U.
+
+  Theorem Expr_Cx : forall {G e T}, Expr G e T -> Cx G.
+  Proof.
+  Admitted.
+
+  Corollary eq_fresh : 
+    forall G D : cx, Cx.eq G D -> 
+    forall x, Cx.isFresh G x -> 
+    Cx.isFresh D x.
+  Admitted.
+
+  Corollary eq_cons : 
+    forall G D : cx, Cx.eq G D ->
+    forall x, Cx.isFresh G x -> 
+    forall T, Cx.eq ((x, T) :: G) ((x, T) :: D).
+  Admitted.
+
+  Hint Resolve eq_fresh eq_cons : core.
+
+  Theorem t_ren :
+    forall {G e T}, Expr G e T ->
+    forall {G'}, Cx G' ->
+    Cx.eq G G' -> Expr G' e T.
+  Proof.
+    induction 1.
+    1,2: constructor; eauto. apply H2. auto.
+    1,4: econstructor; eauto; apply IHExpr2.
+    1,3: econstructor; eauto. 1,2: eapply eq_cons; eauto.
+    1: { econstructor; eauto. apply IHExpr2. econstructor; eauto. 
+         eapply eq_cons; eauto. }
+    all: econstructor; eauto. 
+  Qed.
+
+  Hint Resolve Expr_Cx t_ren : core.
+  (*
+  Fixpoint t_weak 
+    {G e T} (eT : Expr G e T)
+    {W s} (Ws : Expr G W (TSort s))
+    : exists x, Expr ((x, W) :: G) e T.
+  Proof.
+    assert (forall x, Cx.fresh G x -> Cx (G ;; (x, W))). 
+    econstructor; eassumption.
+    destruct eT.
+    - econstructor. constructor. apply H. exact (proj2_sig (unsatur G)).
+    - admit.
+    - econstructor. econstructor. 
+   *)  
+
+  Theorem t_weak :
+    forall {G e T}, Expr G e T ->
+    forall {x W}, Cx ((x, W) :: G) ->
+    Expr ((x, W) :: G) e T.
+  Proof.
+    induction 1.
+    - constructor. auto.
+    - constructor. auto. constructor. auto. admit.
+    - inversion 1; subst. eapply TyAll. 
+      2: apply @t_ren with (G := (x0, W) :: (x, T) :: G). 2: apply IHExpr2.
+      2,3: econstructor. 1,4: apply IHExpr1; eauto. 
+      admit (* TODO: Change to fixpoint? *). admit. admit. admit. admit.
+    - admit.
+    - econstructor. apply IHExpr1; auto. apply IHExpr2; auto. admit.
+    - admit.
+    - econstructor. apply IHExpr1; auto. apply IHExpr2; auto. 
+      apply IHExpr3; auto. admit.
+    - econstructor. apply IHExpr; auto.
+    - econstructor. apply IHExpr; eauto. admit.
+    - econstructor; eauto.
+  Admitted.
+    
+
+
+
